Extract two helper lemmas from existing proof.

concurrency/verif_bst_flows.v
@@ -21,6 +21,15 @@ Definition inset_global_inv (root: TreeNode) (NS: list TreeNode)
 Definition gmap_sub `{Countable K} {A} (s1 s2: gmap K A): Prop :=
   forall k a, s1 !! k = Some a -> s2 !! k = Some a.
 
+Lemma inset_global_inv_perm: forall root l1 l2 I,
+    Permutation l1 l2 -> inset_global_inv root l1 I -> inset_global_inv root l2 I.
+Proof.
+  unfold inset_global_inv. intros. destruct H0 as [? [? ?]]. do 2 (split; auto).
+  apply (Permutation_map key_tn) in H.
+  assert (@list_to_set _ (gset Z) _ _ _ (map key_tn l1) = @list_to_set _ (gset Z) _ _ _ (map key_tn l2)) by
+    now apply list_to_set_perm_L. now rewrite <- H3.
+Qed.
+
 Lemma nzmap_subset_wf: forall `{Countable K} `{CCM A} (s1 s2: gmap K A),
     gmap_sub s1 s2 -> nzmap_wf s2 -> nzmap_wf s1.
 Proof.
@@ -283,6 +292,186 @@ Proof.
   intros. sep_apply tree_rep_impl_pc_tree_rep. apply pc_tree_rep_nodup_addr.
 Qed.
 
+Lemma tree_rep_left_right: forall root l C1 C2,
+    !!(pc_global_inv root l C1) && tree_rep l C1 C2 |--
+             !! (forall x, In x l ->
+                          left_tn x = right_tn x /\ left_tn x = nullval \/ left_tn x ≠ right_tn x).
+Proof.
+  intros. Intros. sep_apply tree_rep_impl_pc_tree_rep.
+  sep_apply (pc_tree_rep_left_right root); auto. Intros.
+  apply prop_right. intros. apply H0; auto.
+Qed.
+
+Lemma tree_rep_inset_cnnt:
+  ∀ (root : TreeNode) (l : list TreeNode) (Cpc : pc_flowint) (Cs : bst_inset_flowint),
+    pc_global_inv root l Cpc → inset_global_inv root l Cs
+    → ∀ (fpc : list pc_flowint) (fs : list bst_inset_flowint),
+        list_join fpc Cpc → list_join fs Cs → length fpc = length l → length fs = length l
+        → iter_sepcon
+            (λ x : TreeNode * (pc_flowint * bst_inset_flowint),
+                node_rep x.1 x.2.1 x.2.2) (combine l (combine fpc fs))
+            |-- !! (∀ x y : TreeNode * (pc_flowint * bst_inset_flowint),
+                       In x (combine l (combine fpc fs)) → In y (combine l (combine fpc fs))
+                       → left_tn x.1 = addr_tn y.1 ∨ right_tn x.1 = addr_tn y.1 → out x.2.2 y.1 = inf y.2.2 y.1).
+Proof.
+  intros. assert (Hit: iter_sepcon
+                 (λ x : TreeNode * (pc_flowint * bst_inset_flowint),
+                     node_rep x.1 x.2.1 x.2.2) (combine l (combine fpc fs)) |-- tree_rep l Cpc Cs). {
+    unfold tree_rep. Exists fpc fs. entailer !. }
+  assert_PROP (∀ x : TreeNode, In x l → x ≠ root →
+                               ∃ y, unique (λ p : TreeNode, In p l ∧ p ≠ x ∧
+                                                              (left_tn p = addr_tn x ∨ right_tn p = addr_tn x)) y). {
+    sep_apply Hit. sep_apply (tree_rep_has_unique_parent root); auto. entailer !. } rename H5 into Hunq.
+  assert_PROP (forall n, In n l -> addr_tn n ≠ nullval). {
+    sep_apply Hit. eapply derives_trans. 2: apply allp_prop_left. apply allp_right. intros. rewrite prop_impl.
+    apply imp_andp_adjoint. Intros.  now apply tree_rep_neq_nullval. } rename H5 into Hnull.
+  assert_PROP (∀ x : TreeNode, In x l → left_tn x ≠ addr_tn root ∧ right_tn x ≠ addr_tn root). {
+    sep_apply Hit. sep_apply (tree_rep_root_no_parent root); auto. entailer !. } rename H5 into Hrnp.
+  assert_PROP (List.NoDup (map addr_tn l)). { sep_apply Hit. sep_apply tree_rep_nodup_addr. entailer !. }
+  rename H5 into Hno. sep_apply tree_rep_local_inv. Intros. apply prop_right. rename H5 into Hloc. intros.
+  destruct (Hloc _ H5). destruct (Hloc _ H6). destruct x as [x [xP xS]]. destruct y as [y [yP yS]].
+  simpl fst in *. simpl snd in *. pose proof (in_combine_r _ _ _ _ H6). apply in_combine_r in H12.
+  apply In_Permutation_cons in H12. destruct H12 as [fsl ?]. eapply list_join_perm in H2; eauto.
+  apply list_join_cons_inv in H2. destruct H2 as [Cl [? ?]]. red in H13.  
+  assert (x ≠ y) by (destruct H8 as [_ [? [? _]]]; intro; subst; destruct H7; exfalso; auto).
+  pose proof (in_combine_r _ _ _ _ H5). apply in_combine_r in H15. eapply Permutation_in in H15; eauto.
+  simpl in H15. destruct H15.
+  - subst. destruct H9 as [_ [? _]]. destruct H11 as [_ [? _]]. rewrite H9 in H11.
+    rewrite set_eq_subseteq in H11. destruct H11. rewrite singleton_subseteq in H11. exfalso. now apply H14.
+  - destruct H0 as [[? ?] [? ?]]. pose proof (intJoin_unfold_inf_1 _ _ _ H13 H0 y).
+    assert (y ∈ domm yS) by (destruct H11 as [? [? ?]]; rewrite H20; now apply elem_of_singleton_2).
+    specialize (H19 H20). pose proof (intJoin_dom _ _ _ H13 H0). pose proof (in_combine_l _ _ _ _ H5).
+    assert (y ∈ domm Cs) by (rewrite H21; rewrite elem_of_union; now left).
+    assert (y ≠ root) by (intro; subst; destruct (Hrnp _ H22); destruct H7; auto). rewrite H18 in H19; auto.
+    rewrite ccm_left_id in H19. apply In_Permutation_cons in H15. destruct H15 as [fsr ?].
+    eapply list_join_perm in H2; eauto. apply list_join_cons_inv in H2. destruct H2 as [Cr [? ?]]. red in H25.
+    assert (✓ Cl) by (apply (intJoin_valid_proj2 _ _ _ H13); auto).
+    assert (y ∉ domm Cl). {
+      assert (intComposable yS Cl) by (eapply intComposable_valid; eauto). destruct H27 as [_ [_ [? _]]]. intro.
+      now apply (H27 y). } rewrite (intJoin_unfold_out _ _ _ H25 H26 _ H27) in H19.
+    assert (✓ Cr) by (apply (intJoin_valid_proj2 _ _ _ H25); auto).
+    assert (y ∉ domm Cr). {
+      pose proof (intJoin_dom _ _ _ H25 H26). intro. apply H27. rewrite H29. rewrite elem_of_union. now right. }
+    rewrite (list_join_unfold_out _ _ H2 H28 _ H29) in H19.
+    assert (forall zS, In zS fsr -> out zS y = ∅). {
+      intros. assert (In zS (yS :: xS :: fsr)) by (now do 2 right).
+      assert (Permutation fs (yS :: xS :: fsr)) by (transitivity (yS :: fsl); auto). symmetry in H32.
+      eapply Permutation_in in H31; eauto. apply (In_snd_combine fpc) in H31. 2: lia. destruct H31 as [zP ?].
+      apply (In_snd_combine l) in H31. 2: rewrite combine_length; lia. destruct H31 as [z ?].
+      destruct (Hloc _ H31) as [_ ?]. simpl in H33. destruct H33 as [? [? [? ?]]]. specialize (H36 y).
+      unfold inset_edgeFn in H36. pose proof (in_combine_l _ _ _ _ H6). pose proof (Hnull _ H37).
+      rewrite <- val_eqb_false in H38. rewrite H38 in H36. clear H38. apply in_combine_l in H31.
+      assert (z ≠ y). {
+        intro. assert (intComposable yS Cl) by (eapply intComposable_valid; eauto). destruct H39 as [_ [_ [? _]]].
+        pose proof (H39 y). specialize (H40 H20). apply H40. rewrite (intJoin_dom xS Cr); auto.
+        apply elem_of_union_r. subst z. pose proof (list_join_dom _ _ H2 H28 _ H30). rewrite elem_of_subseteq in H38.
+        apply H38. rewrite H34. now apply elem_of_singleton_2. } destruct (In_Permutation_cons _ _ H37) as [ly ?].
+      assert (In z ly). { apply (Permutation_in _ H39) in H31. simpl in H31. destruct H31; auto. exfalso; auto. }
+      assert (addr_tn z ≠ addr_tn y). {
+        apply (Permutation_map addr_tn) in H39. apply (Permutation_NoDup H39) in Hno. simpl in Hno.
+        apply NoDup_cons_iff in Hno. destruct Hno as [Hno _]. intro. apply Hno. rewrite <- H41. now apply in_map. }
+      rewrite <- val_eqb_false in H41. rewrite H41 in H36. simpl in H36. clear H41. specialize (Hunq _ H37 H24).
+      destruct Hunq as [yPrnt Huni]. destruct Huni as [_ Huni]. assert (yPrnt = x) by (apply Huni; split; auto).
+      subst yPrnt. assert (x ≠ z). {
+        intro. assert (intComposable xS Cr) by (eapply intComposable_valid; eauto). destruct H42 as [_ [_ [? _]]].
+        pose proof (H42 x). destruct H9 as [_ [? _]]. apply H43.
+        - rewrite H9; now apply elem_of_singleton_2.
+        - subst z. pose proof (list_join_dom _ _ H2 H28 _ H30). rewrite elem_of_subseteq in H41. apply H41.
+          rewrite H34. now apply elem_of_singleton_2. }
+      assert (val_eqb (addr_tn y) (left_tn z) = false). {
+        rewrite val_eqb_false. intro. apply H41. apply Huni; auto. } rewrite H42 in H36.
+      assert (val_eqb (addr_tn y) (right_tn z) = false). {
+        rewrite val_eqb_false. intro. apply H41. apply Huni; auto. } now rewrite H43 in H36. }
+    rewrite accumulate_zero in H19; auto. now rewrite ccm_right_id in H19.
+Qed.
+
+Lemma tree_rep_inset_out:
+  ∀ (root : TreeNode) (l : list TreeNode) (Cpc : pc_flowint) (Cs : bst_inset_flowint),
+    pc_global_inv root l Cpc → inset_global_inv root l Cs
+    → ∀ (fpc : list pc_flowint) (fs : list bst_inset_flowint),
+        list_join fpc Cpc → list_join fs Cs → length fpc = length l → length fs = length l
+        → iter_sepcon
+            (λ x : TreeNode * (pc_flowint * bst_inset_flowint),
+                node_rep x.1 x.2.1 x.2.2) (combine l (combine fpc fs))
+            |-- !! (∀ x y : TreeNode * (pc_flowint * bst_inset_flowint),
+                       In x (combine l (combine fpc fs)) → In y (combine l (combine fpc fs))
+                       → (left_tn x.1 = addr_tn y.1 → out x.2.2 y.1 = split_left (inf x.2.2 x.1) (key_tn x.1)) ∧
+                           (right_tn x.1 = addr_tn y.1 → out x.2.2 y.1 = split_right (inf x.2.2 x.1) (key_tn x.1))).
+Proof.
+  intros. assert (Hit: iter_sepcon
+                 (λ x : TreeNode * (pc_flowint * bst_inset_flowint),
+                     node_rep x.1 x.2.1 x.2.2) (combine l (combine fpc fs)) |-- tree_rep l Cpc Cs). {
+    unfold tree_rep. Exists fpc fs. entailer !. }
+  assert_PROP (forall n, In n l -> addr_tn n ≠ nullval). {
+    sep_apply Hit. eapply derives_trans. 2: apply allp_prop_left. apply allp_right. intros. rewrite prop_impl.
+    apply imp_andp_adjoint. Intros.  now apply tree_rep_neq_nullval. } rename H5 into Hnull.
+  assert_PROP (∀ x : TreeNode, In x l → left_tn x = right_tn x ∧ left_tn x = nullval ∨ left_tn x ≠ right_tn x). {
+    sep_apply Hit. sep_apply (tree_rep_left_right root); auto. entailer !. } rename H5 into Hlr.
+  assert_PROP (List.NoDup (map addr_tn l)). { sep_apply Hit. sep_apply tree_rep_nodup_addr. entailer !. }
+  rename H5 into Hno. sep_apply tree_rep_local_inv. Intros. apply prop_right. rename H5 into Hloc. intros.
+  destruct (Hloc _ H5). destruct (Hloc _ H6). destruct x as [x [xP xS]]. destruct y as [y [yP yS]].
+  simpl fst in *. simpl snd in *. destruct H8 as [? [? [? ?]]]. specialize (H13 y). unfold inset_edgeFn in H13.
+  assert (left_tn x = addr_tn y ∨ right_tn x = addr_tn y → val_eqb (addr_tn x) (addr_tn y) = false). {
+    intros. assert (x ≠ y) by (destruct H7 as [_ [? [? _]]]; intro; subst; destruct H14; auto).
+    apply in_combine_l in H5, H6. apply In_Permutation_cons in H5. destruct H5 as [l' ?].
+    apply (Permutation_in _ H5) in H6. simpl in H6. destruct H6; [now exfalso|].
+    apply (Permutation_map addr_tn) in H5. apply (Permutation_NoDup H5) in Hno. simpl in Hno.
+    apply NoDup_cons_iff in Hno. destruct Hno as [Hno _]. rewrite val_eqb_false. intro. apply Hno.
+    rewrite H16. now apply in_map. }
+  assert (val_eqb (addr_tn y) nullval = false). {
+    intros. apply in_combine_l in H6. apply Hnull in H6. now rewrite val_eqb_false. }
+  split; intros; rewrite H14 in H13; auto; rewrite H15 in H13; simpl in H13.
+  - symmetry in H16. rewrite <- val_eqb_true in H16. now rewrite H16 in H13.
+  - apply in_combine_l in H5. specialize (Hlr _ H5). destruct Hlr as [[? ?] | ?].
+    + rewrite H17 in H18. rewrite H16 in H18. rewrite val_eqb_false in H15. now exfalso.
+    + assert (val_eqb (addr_tn y) (left_tn x) = false). {
+        rewrite val_eqb_false. intro. rewrite H18 in H16. now apply H17. } rewrite H18 in H13.
+      symmetry in H16. rewrite <- val_eqb_true in H16. now rewrite H16 in H13.
+Qed.
+
+Inductive ancestor: TreeNode -> TreeNode -> list TreeNode -> Prop :=
+| ancestor_parent: forall x, ancestor x x (x :: nil)
+| ancestor_more: forall x y z l, left_tn x = addr_tn z \/ right_tn x = addr_tn z ->
+                                 ancestor z y l -> ancestor x y (x :: l).
+
+Lemma tree_rep_root_for_all: forall root l Cpc Cs,
+    !!(pc_global_inv root l Cpc /\ inset_global_inv root l Cs) &&
+      tree_rep l Cpc Cs |--
+               !! (forall x, In x l -> exists sl, ancestor root x sl /\ incl sl l).
+Proof.
+  intros. Intros. sep_apply (tree_rep_has_unique_parent root); auto. Intros. rename H1 into Huni.
+  sep_apply tree_rep_nodup_addr. Intros. rename H1 into Hno.
+  assert_PROP (forall n, In n l -> addr_tn n ≠ nullval). {
+    eapply derives_trans. 2: apply allp_prop_left. apply allp_right. intros. rewrite prop_impl.
+    apply imp_andp_adjoint. Intros.  now apply tree_rep_neq_nullval. } rename H1 into Hnull.
+  sep_apply (tree_rep_left_right root); auto. Intros. rename H1 into Hlr. unfold tree_rep. Intros fpc fs.
+  sep_apply (tree_rep_inset_cnnt root l Cpc Cs). Intros. rename H5 into Hcnt.
+  sep_apply (tree_rep_inset_out root l Cpc Cs). Intros. rename H5 into Hout. sep_apply tree_rep_local_inv. Intros.
+  apply prop_right.
+  assert (forall x y, In x (combine l (combine fpc fs)) -> In y (combine l (combine fpc fs)) ->
+                      left_tn x.1 = addr_tn y.1 \/ right_tn x.1 = addr_tn y.1 ->
+                      inset y.2.2 y.1 ⊂ inset x.2.2 x.1). { admit. } intros. destruct (treenode_eq_dec x root).
+  - subst. exists (root :: nil). split. 1: constructor. destruct H as [? [? [? [? ?]]]].
+    repeat intro. simpl in H12. destruct H12; try easy. now subst.
+  -
+Abort.
+
+Lemma tree_rep_inset_range:
+  forall (l : list TreeNode) (Cpc : pc_flowint) (Cs : bst_inset_flowint)
+         (fpc : list pc_flowint) (fs : list bst_inset_flowint) root,
+    list_join fpc Cpc -> list_join fs Cs -> length fpc = length l ->
+    length fs = length l -> pc_global_inv root l Cpc ->
+    inset_global_inv root l Cs ->
+    (forall x, In x (combine l (combine fpc fs)) ->
+               pc_local_inv x.1 x.2.1 /\ inset_local_inv x.1 x.2.2) ->
+    forall x xI xS y yI yS z,
+      In (x, (xI, xS)) (combine l (combine fpc fs)) ->
+      In (y, (yI, yS)) (combine l (combine fpc fs)) -> x ≠ y ->
+      in_inset z xS x -> in_inset z yS y -> ancestor x y l \/ ancestor y x l.
+Proof.
+  intros.
+Abort.
+
 Definition lookup_inv (root: TreeNode) (b: val) (l: list TreeNode)
            (Cpc : pc_flowint) (Cs: bst_inset_flowint) (x: Z): environ -> mpred :=
   EX n: TreeNode, EX l': list TreeNode, EX nI: pc_flowint, EX Cl: pc_flowint,
@@ -297,13 +486,15 @@ Definition lookup_inv (root: TreeNode) (b: val) (l: list TreeNode)
                           if Val.eq (addr_tn n) nullval then emp else node_rep n nI nS;
                           tree_rep l' Cl Cls).
 
+
 Lemma body_lookup: semax_body Vprog Gprog f_lookup lookup_spec.
 Proof.
   start_function.
   unfold treebox_rep. Intros. sep_apply (tree_rep_has_children root l Cpc Cs); auto.
   Intros. sep_apply (tree_rep_root_no_parent root); auto. Intros. rename H4 into Hr.
   sep_apply tree_rep_nodup_addr. Intros. rename H4 into Hno.
-  sep_apply (tree_rep_has_unique_parent root); auto. Intros. rename H4 into Huni. forward.
+  sep_apply (tree_rep_has_unique_parent root); auto. Intros. rename H4 into Huni.
+  sep_apply (tree_rep_left_right root); auto. Intros. rename H4 into Hlr. forward.
   - entailer. sep_apply (tree_rep_saturate_local root l Cpc Cs); auto. entailer !.
   - forward_while (lookup_inv root b l Cpc Cs x).
     + Exists root. destruct H1 as [_ [_ [_ [? _]]]].
@@ -332,7 +523,7 @@ Proof.
         -- Exists (empty_node, l, ∅ : pc_flowint, Cpc, ∅ : bst_inset_flowint, Cs). simpl fst. simpl snd.
            if_tac. 2: cbn in H15; now exfalso. clear H15. entailer. apply andp_right. 2: sep_apply H12; entailer !.
            unfold tree_rep. Intros fpc fs. sep_apply tree_rep_local_inv. Intros. apply prop_right.
-           split; [|split]; [apply intJoin_left_unit..|]. 
+           split; [|split]; [apply intJoin_left_unit..|]. destruct H9 as [? [? [? [? [? [? [? ?]]]]]]].
            rewrite Int.signed_repr in H14; auto.
         (* if the key was in some other node, then it would be removed from
            the inset of all that node's descendants, contradicting the assumption
@@ -340,7 +531,7 @@ Proof.
            intro. apply list_in_map_inv in H32. destruct H32 as [xN [? ?]].
            assert (In xN l'). {
             symmetry in H10. apply (Permutation_in xN H10) in H33. destruct H33; auto. subst. lia. }
-          admit. 
+          admit.
         -- rewrite H16. assert (In p l'). {
             symmetry in H10. apply Permutation_in with (l' := n :: l') in H3; auto.
             simpl in H3. destruct H3; auto. symmetry in H3. now exfalso. }
@@ -349,77 +540,33 @@ Proof.
            apply intJoin_comm in H4, H5. destruct (intJoin_assoc _ _ _ _ _ H19 H4) as [pIpc [? ?]].
            destruct (intJoin_assoc _ _ _ _ _ H20 H5) as [pSs [? ?]].
            Exists (p, (n :: pl), pI, pIpc, pS, pSs). simpl fst. simpl snd. if_tac.
-           1: now exfalso. unfold node_rep. Intros. unfold tree_rep at 1.
-           Intros fpc fs. sep_apply tree_rep_local_inv. Intros. entailer !.
-           ++ split. 2: transitivity (n :: p :: pl);
-                     [apply perm_swap | transitivity (n :: l'); auto].
-              destruct H9 as [? [? [? [? [? [? [? ?]]]]]]].
-              rewrite Int.signed_repr in H14; auto. destruct H8 as [? [? [? ?]]].
-              specialize (H50 p). unfold inset_edgeFn in H50. red.
-              rewrite <- H16 in H50. rewrite <- val_eqb_false in H41.
-              rewrite H41 in H50. rewrite <- H16 in H18.
-              rewrite <- val_eqb_false in H18. rewrite H18 in H50. simpl in H50.
-              rewrite val_eqb_refl in H50. red in H6. apply nzmap_elem_of_dom in H6.
-              red in H6. assert (p ≠ root). {
-               intro. subst p. destruct (Hr _ H11). auto. }
-             destruct H6 as [a ?].
-              assert (x ∈ dom_ms (out nS p)). {
-               rewrite nzmap_elem_of_dom. exists a. rewrite H50.
-               apply split_left_lookup. split; auto. }
-             assert (inf pS p = out nS p). {
-               destruct H2 as [[? ?] [? ?]]. destruct H27 as [_ [? _]].
-               pose proof (intJoin_unfold_inf_1 _ _ _ H25 H2 p).
-               assert (p ∈ domm pS). {
-                 rewrite H27. now apply elem_of_singleton_2. } specialize (H56 H57).
-               pose proof (intJoin_dom _ _ _ H25 H2).
-               assert (p ∈ domm Cs). {
-                 rewrite H58. rewrite elem_of_union. now left. }
-               rewrite H55 in H56; auto. rewrite ccm_left_id in H56.
-               assert (✓ pSs) by (apply (intJoin_valid_proj2 _ _ _ H25); auto).
-               assert (p ∉ domm pSs). {
-                 assert (intComposable pS pSs) by
-                   (eapply intComposable_valid; eauto).
-                 destruct H61 as [_ [_ [? _]]]. intro. now apply (H61 p). }
-               rewrite (intJoin_unfold_out _ _ _ H24 H60 _ H61) in H56.
-               assert (✓ pCls) by (apply (intJoin_valid_proj1 _ _ _ H24); auto).
-               assert (p ∉ domm pCls). {
-                 pose proof (intJoin_dom _ _ _ H24 H60). intro. apply H61.
-                 rewrite H63. rewrite elem_of_union. now left. }
-               rewrite (list_join_unfold_out _ _ H30 H62 _ H63) in H56.
-               assert (forall yS, In yS fs -> out yS p = ∅). {
-                 intros. apply (In_snd_combine fpc) in H64. 2: lia.
-                 destruct H64 as [yP ?]. apply (In_snd_combine pl) in H64.
-                 2: rewrite combine_length; lia. destruct H64 as [y ?].
-                 specialize (H33 _ H64). destruct H33 as [_ ?]. simpl in H33.
-                 destruct H33 as [? [? [? ?]]]. specialize (H67 p). unfold inset_edgeFn in H67.
-                 rewrite <- val_eqb_false in H26. rewrite H26 in H67. apply in_combine_l in H64.
-                 assert (addr_tn y ≠ addr_tn p). {
-                   apply (Permutation_map addr_tn) in H10.
-                   symmetry in H10. apply (Permutation_NoDup H10) in Hno. simpl in Hno.
-                   apply NoDup_cons_iff in Hno. destruct Hno as [_ Hno].
-                   apply (Permutation_map addr_tn) in H21. symmetry in H21.
-                   apply (Permutation_NoDup H21) in Hno. simpl in Hno.
-                   apply NoDup_cons_iff in Hno. destruct Hno as [Hno _].
-                   intro. apply Hno. rewrite <- H68. now apply in_map. }
-                 rewrite <- val_eqb_false in H68. rewrite H68 in H67. simpl in H67.
-                 specialize (Huni _ H3 H51). destruct Huni as [pRoot Huni]. destruct Huni as [_ Huni].
-                 assert (pRoot = n) by (apply Huni; split; auto). subst pRoot.
-                 assert (In y l). {
-                   eapply Permutation_in; eauto. right. eapply Permutation_in; eauto. now right. }
-                 assert (y ≠ p). {
-                   apply val_eqb_false in H68. intro. apply H68. now subst. }
-                 assert (n ≠ y). {
-                   intro. subst y. apply (in_cons p n) in H64. apply (Permutation_in n H21) in H64.
-                   apply NoDup_map_inv in Hno. symmetry in H10. apply (Permutation_NoDup H10) in Hno.
-                   apply NoDup_cons_iff in Hno. now destruct Hno. }
-                 assert (val_eqb (addr_tn p) (left_tn y) = false). {
-                   rewrite val_eqb_false. intro. apply H71. apply Huni; auto. } rewrite H72 in H67.
-                 assert (val_eqb (addr_tn p) (right_tn y) = false). {
-                   rewrite val_eqb_false. intro. apply H71. apply Huni; auto. } now rewrite H73 in H67. }
-               rewrite accumulate_zero in H56; auto. now rewrite ccm_left_id in H56. } now rewrite H53.
-           ++ rewrite tree_rep_cons. Exists nI nS pClpc pCls.
-              apply intJoin_comm in H22, H24. unfold tree_rep. Exists fpc fs.
-              unfold node_rep. rewrite <- H16. entailer !.
+           1: now exfalso. unfold tree_rep at 1. Intros fpc fs. sep_apply tree_rep_local_inv. Intros.
+           gather_SEP (iter_sepcon _ _) (node_rep _ _ _) (data_at Tsh t_struct_tree _ (addr_tn n)).
+           replace_SEP 0 (iter_sepcon (λ y, node_rep y.1 y.2.1 y.2.2)
+                                      (combine (p :: n :: pl) (combine (pI :: nI :: fpc) (pS :: nS :: fs)))). {
+            entailer !. simpl combine. simpl iter_sepcon. cancel. unfold node_rep. rewrite <- H16. entailer !. }
+          assert (p :: n :: pl ≡ₚ l). {
+            transitivity (n :: p :: pl); [apply perm_swap | transitivity (n :: l'); auto]. } symmetry in H32.
+           assert (pc_global_inv root (p :: n :: pl) Cpc) by (eapply pc_global_inv_perm; eauto).
+           assert (inset_global_inv root (p :: n :: pl) Cs) by (eapply inset_global_inv_perm; eauto).
+           assert (list_join (pI :: nI :: fpc) Cpc). {
+            apply join_cons with pIpc; auto. apply intJoin_comm in H22. apply join_cons with pClpc; auto. }
+          assert (list_join (pS :: nS :: fs) Cs). {
+            apply join_cons with pSs; auto. apply intJoin_comm in H24. apply join_cons with pCls; auto. }
+          assert (length (pI :: nI :: fpc) = length (p :: n :: pl)) by (simpl; auto).
+           assert (length (pS :: nS :: fs) = length (p :: n :: pl)) by (simpl; auto).
+           sep_apply (tree_rep_inset_cnnt root (p :: n :: pl) Cpc Cs); auto. Intros.
+           sep_apply (tree_rep_inset_out root (p :: n :: pl) Cpc Cs); auto. Intros.
+           assert (In (p, (pI, pS)) (combine (p :: n :: pl)
+                                             (combine (pI :: nI :: fpc) (pS :: nS :: fs)))) by (simpl; now left).
+           assert (In (n, (nI, nS)) (combine (p :: n :: pl) (combine (pI :: nI :: fpc) (pS :: nS :: fs)))). {
+            simpl. right. now left. } specialize (H39 _ _ H42 H41). specialize (H40 _ _ H42 H41). simpl in H39, H40.
+           destruct H40. specialize (H39 (or_introl H16)). specialize (H40 H16). symmetry in H32. entailer !.
+           ++ red in H6. apply nzmap_elem_of_dom in H6. red in H6. destruct H6 as [a ?].
+              red. rewrite <- H39. rewrite H40. rewrite nzmap_elem_of_dom. exists a.
+              apply split_left_lookup. destruct H9 as [? _]. rewrite Int.signed_repr in H14; auto.
+           ++ simpl iter_sepcon. cancel. rewrite tree_rep_cons. Exists nI nS pClpc pCls.
+              apply intJoin_comm in H22, H24. unfold tree_rep. Exists fpc fs. entailer !.
       * forward_if.
         -- forward; destruct H13 as [? | [p [? [? ?]]]].
            ++ rewrite H13; entailer !.
@@ -431,80 +578,35 @@ Proof.
              sep_apply (tree_rep_neq_nullval p l' Cl Cls). Intros.
               rewrite (tree_rep_In_eq p l' Cl Cls); auto. Intros pI pS pl pClpc pCls.
               apply intJoin_comm in H4, H5. destruct (intJoin_assoc _ _ _ _ _ H20 H4) as [pIpc [? ?]].
-              destruct (intJoin_assoc _ _ _ _ _ H21 H5) as [pSs [? ?]].
-              Exists (p, (n :: pl), pI, pIpc, pS, pSs). simpl fst. simpl snd. if_tac.
-              1: now exfalso. unfold node_rep. Intros. unfold tree_rep at 1.
-              Intros fpc fs. sep_apply tree_rep_local_inv. Intros. entailer !.
-              ** split. 2: transitivity (n :: p :: pl);
-                        [apply perm_swap | transitivity (n :: l'); auto].
-                 destruct H9 as [? [? [? [? [? [? [? ?]]]]]]].
-                 rewrite Int.signed_repr in H15; auto. destruct H8 as [? [? [? ?]]].
-                 specialize (H51 p). unfold inset_edgeFn in H51. red.
-                 rewrite <- H17 in H51. rewrite <- val_eqb_false in H43.
-                 rewrite H43 in H51. rewrite <- H17 in H19.
-                 rewrite <- val_eqb_false in H19. rewrite H19 in H51. simpl in H51.
-                 rewrite val_eqb_refl in H51.
-                 assert (val_eqb (right_tn n) (left_tn n) = false) as Hlrn. {
-                  admit. } rewrite Hlrn in H51. clear Hlrn. red in H6. apply nzmap_elem_of_dom in H6.
-                 red in H6. assert (p ≠ root). {
-                  intro. subst p. destruct (Hr _ H11). auto. }
-                destruct H6 as [a ?]. assert (x ∈ dom_ms (out nS p)). {
-                  rewrite nzmap_elem_of_dom. exists a. rewrite H51.
-                  apply split_right_lookup. split; auto. lia. }
-                assert (inf pS p = out nS p). {
-                  destruct H2 as [[? ?] [? ?]]. destruct H28 as [_ [? _]].
-                  pose proof (intJoin_unfold_inf_1 _ _ _ H26 H2 p).
-                  assert (p ∈ domm pS). {
-                    rewrite H28. now apply elem_of_singleton_2. } specialize (H57 H58).
-                  pose proof (intJoin_dom _ _ _ H26 H2).
-                  assert (p ∈ domm Cs). {
-                    rewrite H59. rewrite elem_of_union. now left. }
-                  rewrite H56 in H57; auto. rewrite ccm_left_id in H57.
-                  assert (✓ pSs) by (apply (intJoin_valid_proj2 _ _ _ H26); auto).
-                  assert (p ∉ domm pSs). {
-                    assert (intComposable pS pSs) by
-                      (eapply intComposable_valid; eauto).
-                    destruct H62 as [_ [_ [? _]]]. intro. now apply (H62 p). }
-                  rewrite (intJoin_unfold_out _ _ _ H25 H61 _ H62) in H57.
-                  assert (✓ pCls) by (apply (intJoin_valid_proj1 _ _ _ H25); auto).
-                  assert (p ∉ domm pCls). {
-                    pose proof (intJoin_dom _ _ _ H25 H61). intro. apply H62.
-                    rewrite H64. rewrite elem_of_union. now left. }
-                  rewrite (list_join_unfold_out _ _ H31 H63 _ H64) in H57.
-                  assert (forall yS, In yS fs -> out yS p = ∅). {
-                    intros. apply (In_snd_combine fpc) in H65. 2: lia.
-                    destruct H65 as [yP ?]. apply (In_snd_combine pl) in H65.
-                    2: rewrite combine_length; lia. destruct H65 as [y ?].
-                    specialize (H34 _ H65). destruct H34 as [_ ?]. simpl in H34.
-                    destruct H34 as [? [? [? ?]]]. specialize (H68 p). unfold inset_edgeFn in H68.
-                    rewrite <- val_eqb_false in H27. rewrite H27 in H68. apply in_combine_l in H65.
-                    assert (addr_tn y ≠ addr_tn p). {
-                      apply (Permutation_map addr_tn) in H10.
-                      symmetry in H10. apply (Permutation_NoDup H10) in Hno. simpl in Hno.
-                      apply NoDup_cons_iff in Hno. destruct Hno as [_ Hno].
-                      apply (Permutation_map addr_tn) in H22. symmetry in H22.
-                      apply (Permutation_NoDup H22) in Hno. simpl in Hno.
-                      apply NoDup_cons_iff in Hno. destruct Hno as [Hno _].
-                      intro. apply Hno. rewrite <- H69. now apply in_map. }
-                    rewrite <- val_eqb_false in H69. rewrite H69 in H68. simpl in H68.
-                    specialize (Huni _ H13 H52). destruct Huni as [pRoot Huni]. destruct Huni as [_ Huni].
-                    assert (pRoot = n) by (apply Huni; split; auto). subst pRoot.
-                    assert (In y l). {
-                      eapply Permutation_in; eauto. right. eapply Permutation_in; eauto. now right. }
-                    assert (y ≠ p). {
-                      apply val_eqb_false in H69. intro. apply H69. now subst. }
-                    assert (n ≠ y). {
-                      intro. subst y. apply (in_cons p n) in H65. apply (Permutation_in n H22) in H65.
-                      apply NoDup_map_inv in Hno. symmetry in H10. apply (Permutation_NoDup H10) in Hno.
-                      apply NoDup_cons_iff in Hno. now destruct Hno. }
-                    assert (val_eqb (addr_tn p) (left_tn y) = false). {
-                      rewrite val_eqb_false. intro. apply H72. apply Huni; auto. } rewrite H73 in H68.
-                    assert (val_eqb (addr_tn p) (right_tn y) = false). {
-                      rewrite val_eqb_false. intro. apply H72. apply Huni; auto. } now rewrite H74 in H68. }
-                  rewrite accumulate_zero in H57; auto. now rewrite ccm_left_id in H57. } now rewrite H54.
-              ** rewrite tree_rep_cons. Exists nI nS pClpc pCls.
-                 apply intJoin_comm in H23, H25. unfold tree_rep. Exists fpc fs.
-                 unfold node_rep. rewrite <- H17. entailer !.
+              destruct (intJoin_assoc _ _ _ _ _ H21 H5) as [pSs [? ?]]. Exists (p, (n :: pl), pI, pIpc, pS, pSs).
+              simpl fst. simpl snd. if_tac. 1: now exfalso. unfold tree_rep at 1. Intros fpc fs.
+              sep_apply tree_rep_local_inv. Intros.
+              gather_SEP (iter_sepcon _ _) (node_rep _ _ _) (data_at Tsh t_struct_tree _ (addr_tn n)).
+              replace_SEP 0 (iter_sepcon (λ y, node_rep y.1 y.2.1 y.2.2)
+                                      (combine (p :: n :: pl) (combine (pI :: nI :: fpc) (pS :: nS :: fs)))). {
+            entailer !. simpl combine. simpl iter_sepcon. cancel. unfold node_rep. rewrite <- H17. entailer !. }
+          assert (p :: n :: pl ≡ₚ l). {
+            transitivity (n :: p :: pl); [apply perm_swap | transitivity (n :: l'); auto]. } symmetry in H33.
+           assert (pc_global_inv root (p :: n :: pl) Cpc) by (eapply pc_global_inv_perm; eauto).
+           assert (inset_global_inv root (p :: n :: pl) Cs) by (eapply inset_global_inv_perm; eauto).
+           assert (list_join (pI :: nI :: fpc) Cpc). {
+            apply join_cons with pIpc; auto. apply intJoin_comm in H23. apply join_cons with pClpc; auto. }
+          assert (list_join (pS :: nS :: fs) Cs). {
+            apply join_cons with pSs; auto. apply intJoin_comm in H25. apply join_cons with pCls; auto. }
+          assert (length (pI :: nI :: fpc) = length (p :: n :: pl)) by (simpl; auto).
+           assert (length (pS :: nS :: fs) = length (p :: n :: pl)) by (simpl; auto).
+           sep_apply (tree_rep_inset_cnnt root (p :: n :: pl) Cpc Cs); auto. Intros.
+           sep_apply (tree_rep_inset_out root (p :: n :: pl) Cpc Cs); auto. Intros.
+           assert (In (p, (pI, pS)) (combine (p :: n :: pl)
+                                             (combine (pI :: nI :: fpc) (pS :: nS :: fs)))) by (simpl; now left).
+           assert (In (n, (nI, nS)) (combine (p :: n :: pl) (combine (pI :: nI :: fpc) (pS :: nS :: fs)))). {
+            simpl. right. now left. } specialize (H40 _ _ H43 H42). specialize (H41 _ _ H43 H42). simpl in H41, H40.
+           destruct H41. specialize (H40 (or_intror H17)). specialize (H44 H17). symmetry in H33. entailer !.
+           ** red in H6. apply nzmap_elem_of_dom in H6. red in H6. destruct H6 as [a ?].
+              red. rewrite <- H40. rewrite H44. rewrite nzmap_elem_of_dom. exists a. apply split_right_lookup.
+              destruct H9 as [? _]. rewrite Int.signed_repr in H15; auto. split; auto. lia.
+           ** simpl iter_sepcon. cancel. rewrite tree_rep_cons. Exists nI nS pClpc pCls.
+              apply intJoin_comm in H23, H25. unfold tree_rep. Exists fpc fs. entailer !.
         -- forward; destruct H9 as [? [? [? [? [? [? [? ?]]]]]]].
            ++ entailer !.
            ++ sep_apply H12. forward. Exists (value_tn n). unfold treebox_rep.
